theories/FSets/OrderedType.v
@@ -313,6 +313,8 @@ Ltac false_order := elimtype False; order.
 
 (* Specialization of resuts about lists modulo. *)
 
+Section ForNotations.
+
 Notation In:=(InA eq).
 Notation Inf:=(lelistA lt).
 Notation Sort:=(sort lt).
@@ -345,6 +347,8 @@ Proof. exact (InfA_alt eq_refl eq_sym lt_trans lt_eq eq_lt). Qed.
 
 Lemma Sort_NoDup : forall l, Sort l -> NoDup l.
 Proof. exact (SortA_NoDupA eq_refl eq_sym lt_trans lt_not_eq lt_eq eq_lt) . Qed.
+
+End ForNotations.
 
 Hint Resolve ListIn_In Sort_NoDup Inf_lt. 
 Hint Immediate In_eq Inf_lt. 
